Made room for an updated Lab 2.

lab8/src/main.cpp
@@ -1,15 +1,10 @@
-#include <iostream>
 
-#include "scanner.h"
+#include "minotaur.h"
 
 
 int main(int argc, char *argv[]) {
-    std::string s;
-    bool result;
-    while(1) {
-        std::getline(std::cin, s);
-        ANONYMOUS::match(s.size(), (char*)s.c_str(), result);
-        std::cout << " = " << result << std::endl;
-    }
+
+    ANONYMOUS::escape__Wrapper();
+
 }
 
