lab9/src/main.cpp
@@ -1,39 +1,15 @@
 #include <iostream>
 
-#include "listops.h"
-
-
-
-using listops::Node;
-
-
-Node * list_from_args(int argc, char *argv[]) {
-    int vals[argc];
-
-    for (int i = 0; i < argc; i++)
-        vals[i] = atoi(argv[i]);
-
-    Node *h;
-    listops::mklist(argc-1, vals, h);
-
-    return h;
-}
-
-void print_list(Node *h) {
-    for ( ; h != NULL; h = h->next)
-        std::cout << h->val << " ";
-    std::cout << std::endl;
-}
+#include "scanner.h"
 
 
 int main(int argc, char *argv[]) {
-
-    Node *h = list_from_args(argc-1, argv+1);
-
-    print_list(h);
-
-    listops::reverse(h, h);
-
-    print_list(h);
+    std::string s;
+    bool result;
+    while(1) {
+        std::getline(std::cin, s);
+        ANONYMOUS::match(s.size(), (char*)s.c_str(), result);
+        std::cout << " = " << result << std::endl;
+    }
 }
 
