lab6/extra/demo-factorial.v
@@ -1,0 +1,131 @@
+Require Import Arith.
+Require Import Omega.
+Import Nat.
+
+
+Load "./hoare".
+
+
+(* From "Formal Reasoning About Programs"
+
+   factorial(n) {
+      a = 1;
+      while (n > 0) {
+         a = a * n;
+         n = n - 1;
+      }
+      return a; 
+   }
+*)
+
+Definition gt01 n m := if gt_dec n m then 1 else 0.
+
+Notation "[ e1 `*` e2 ]" := (expr_op e1 mul e2).
+Notation "[ e1 `-` e2 ]" := (expr_op e1 sub e2).
+Notation "[ e1 `>` e2 ]" := (expr_op e1 gt01 e2).
+
+Notation "$ v" := (expr_var v) (at level 7, format "$ v").
+Notation "# n" := (expr_num n) (at level 7, format "# n").
+
+
+Definition factorial_cmd :=
+  seq (assign a (#1))
+      (while [$n `>` #0]
+             (seq (assign a [$a `*` $n])
+                  (assign n [$n `-` #1]))).
+
+
+
+Module MainProof.
+
+  Definition c := seq (assign a [$a `*` $n])
+                      (assign n [$n `-` #1]).
+
+  (* Loop invariant:  a * n! = n0!  *)
+  Definition linv n0 (s : state) := s a * fact (s n) = fact n0.
+
+  (* Control the behavior of `simpl` to allow more unfoldings.            *)
+  (*                                                                      *)
+  (* This should allow you to simplify a substitution term,               *)
+  (*   e.g. subst (fun s => s a + 1 = 2) a [$a `-` #1] s                  *)
+  (*        ( in other words, (a + 1 = 2)[a - 1 / a] )                    *)
+  (*     simplifies to                                                    *)
+  (*        s a - 1 + 1 = 2                                               *)
+  Arguments subst P v e /.
+  Arguments set s v / z.
+  Arguments var_eq_dec !v1 !v2.
+  Arguments gt01 n m / : simpl nomatch.
+
+  (*                                     *)
+  (*  { linv /\ n > 0 }  c  { linv }     *)
+  (*                                     *)
+  (* or:                                 *)
+  (*                                     *)
+  (*  { a * n! = n0 /\ n > 0 }           *)
+  (*  a := a * n ; n := n - 1            *)
+  (*  { a * n! = n0 }                    *)
+  (*                                     *)
+  Lemma factorial_inv n0 : hoare (fun s => linv n0 s /\ s n > 0)
+                                 c
+                                 (linv n0).
+  Proof.
+    unfold c. unfold linv. eapply hoare_seq.
+    Focus 2. apply hoare_assign.
+    simpl.
+    eapply hoare_weaken_l.
+    Focus 2. apply hoare_assign.
+    simpl.
+    (* now it's just a game of arithmetics *)
+    firstorder.
+    destruct (s n).
+    - inversion H0.
+    - simpl.
+      rewrite sub_0_r. rewrite <- mul_assoc. assumption.
+  Qed.
+  
+  Lemma gt0_le x y : gt01 x y = 0 <-> x <= y.  Admitted.
+  Lemma gt1_gt x y : gt01 x y <> 0 <-> x > y.  Admitted.
+
+  (*                                                       *)
+  (*  { linv }  while (n > 0) do c  { linv /\ n <= 0 }     *)
+  (*                                                       *)
+  Lemma factorial_inv' n0 : hoare (linv n0)
+                                  (while [$n `>` #0] c)
+                                  (fun s => linv n0 s /\ s n = 0).
+  Proof.
+    eapply hoare_weaken_r.
+    - econstructor. simpl. eapply hoare_weaken_l.
+      + intros. rewrite gt1_gt in H. apply H.
+      + apply factorial_inv.
+    - simpl. intros. firstorder.
+      apply gt0_le in H0. omega.
+  Qed.
+
+  Lemma final n0 s : linv n0 s -> s n = 0 -> s a = fact n0.
+  Admitted.
+
+  (*                                                 *)
+  (*     { n = n0 }  factorial  { a = n0! }          *)
+  (*                                                 *)
+  Lemma factorial_correct n0 : hoare (fun s => s n = n0)
+                                     factorial_cmd
+                                     (fun s => s a = fact n0).
+  Proof.
+    econstructor.
+    Focus 2.
+    { eapply hoare_weaken_r.
+      - apply factorial_inv'.
+      - simpl. intros. apply final; apply H.
+    }
+    Unfocus.
+    (*  { n = n0 }  a := 1  { a * n! = n0! }  *)
+    eapply hoare_weaken_l.
+    Focus 2. constructor.
+    intros. unfold linv. simpl. rewrite H. omega.
+  Qed.
+
+End MainProof.
+
+
+
+
